---
title: 一
tags:
  - 数至十
---

<!-- <script src="https://cdnjs.cloudflare.com/ajax/libs/mathjax/2.7.5/MathJax.js?config=TeX-AMS_HTML" async></script> -->
![alt text](https://pic3.zhimg.com/80/v2-676d16d629cb37c4b544e641adc4da4e_1440w.webp)

$\displaystyle\lim_{n\rightarrow\infty}\frac{2^{-n}}{n(n+1)}\sum_{k=1}^{n}C_{n}^{k}・k^2$

**解：**  

$$\displaystyle\because(1+x)^n=\sum_{k=0}^{n}C_{n}^{k}・x^k$$  

$\displaystyle\therefore$
对二项式$\displaystyle(1+x)^n=\sum_{k=0}^{n}C_{n}^{k}・x^k$两边求导：

$$\displaystyle n(1+x)^{n-1}=\sum_{k=0}^{n}C_{n}^{k}・kx^{k-1}$$

两边同时乘以$x$：
<center>

$\displaystyle nx(1+x)^{n-1}=\sum_{k=1}^{n}C_{n}^{k}・kx^k$  
</center>

两边再次求导：  

$$\displaystyle n(1+x)^{n-1}+nx(n-1)(1+x)^{n-2}=\sum_{k=1}^{n}C_{n}^{k}・k^2x^{k-1}$$  

令$x=1$：  

$$\displaystyle \sum_{k=1}^{n}C_{n}^{k}・k^2=n(n+2)・2^{n-2}$$  

$\therefore$ 
$\displaystyle\lim_{n\rightarrow\infty}\frac{2^{-n}}{n(n+1)}\sum_{k=1}^{n}C_{n}^{k}・k^2=\lim_{n\rightarrow\infty}\frac{2^{-n}}{n(n+1)}n(n+2)2^{n-2}=\frac{1}{4}$
