---
title: 二
tags:
  - 数至十
---

<!-- <script src="https://cdnjs.cloudflare.com/ajax/libs/mathjax/2.7.5/MathJax.js?config=TeX-AMS_HTML" async></script> -->
## 芝士点
**轮换和(Cyclic Sum): 考虑一个函数$f(x_1,x_2,\cdots,x_n)$，它的轮换和定义为**

$\displaystyle\sum _{cyc}f(x_1,x_2,\cdots,x_n)=f(x_1,x_2,\cdots,x_{n-1},x_n)+f(x_2,x_3\cdots,x_n,x_1)+\cdots +f(x_n,x_1,\cdots,x_{n-2},x_{n-1})$  

![img](https://cn.mcecy.com/image/20230621/0a509d78a82508ea411f433b093ec036.png)
***

## 例题

**正实数x,y,z满足$xyz\ge1$，证明$\displaystyle\frac{x^5-x^2}{x^5+y^2+z^2}+\frac{y^5-y^2}{x^2+y^5+z^2}+\frac{z^5-z^2}{x^2+y^2+z^5} \ge 0$**  

**解：**  

$\because$  $\displaystyle\frac{x^5-x^2}{x^5+y^2+z^2}-\frac{x^5-x^2}{x^3(x^5+y^2+z^2)}=\frac{x^5-x^2}{x^3(x^5+y^2+z^2)(x^2+y^2+z^2)}\ge0$

$\therefore$  $\displaystyle\sum _{cyc}\frac{x^5-x^2}{x^5+y^2+z^2}\ge\sum _{cyc}\frac{x^5-x^2}{x^3(x^2+y^2+z^2)}=\frac{1}{x^2+y^2+z^2}\sum _{cyc}(x^2-\frac{1}{x})\ge\frac{1}{x^2+y^2+z^2}\sum _{cyc}(x^2-yz)\ge0$  
**得证**

题源：2005-46th-IMO-3